p(x)\qquad \qquad \qquad \qquad \qquad \qquad \qquad \qquad \qquad \qquad \\ { p }_{ new }(x)\quad \sim \quad N(\mu ,v)\\ \\ { E }[x]\\ { E }[{ x }^{ 2 }]\\ \\ { E }_{ p }[x]\quad =\quad { E }_{ p\_ new }[x]\\ { E }_{ p }[{ x }^{ 2 }]\quad =\quad { E }_{ p\_ new }[{ x }^{ 2 }]\\ { \mu  }_{ p\_ new }\quad =\quad { E }_{ p }[x]\\ { v }_{ p\_ new }\quad =\quad { E }_{ p }[{ x }^{ 2 }]\quad -\quad { { E }_{ p }[x] }^{ 2 }\\ \\ p(x)\quad =\quad \frac { f(x)q(x) }{ Z(\mu ,v) } \\ q(x)\quad \sim \quad N(\mu ,v)\\ Z(\mu ,v)\quad =\quad \int { f(x)q(x)d(x) } \\ \\ { E }_{ p }[x]\quad =\quad \mu \quad +\quad { v\triangledown  }_{ \mu  }\log { Z(\mu ,v) } \\ { E }_{ p }[{ x }^{ 2 }]\quad =\quad 2{ v }^{ 2 }{ \triangledown  }_{ v }\log { Z } \quad +\quad v\quad +\quad { \mu  }^{ 2 }\quad +\quad 2v\mu { \triangledown  }_{ \mu  }\log { Z } \\ { \mu  }_{ p\_ new }\quad =\quad { E }_{ p }[x]\quad =\quad \mu \quad +\quad \sigma { v\triangledown  }_{ \mu  }\log { Z(\mu ,v) } \\ { v }_{ p\_ new }\quad =\quad { E }_{ p }[{ x }^{ 2 }]\quad -\quad { { E }_{ p }[x] }^{ 2 }\quad =\quad v\quad -\quad v({ { \triangledown  }_{ \mu  } }^{ 2 }\quad -\quad 2{ \triangledown  }_{ v }\log { Z } )v\\ \\ p(x|\eta )\quad =\quad h(x)g(\eta )exp\{ { \eta  }^{ T }u(x)\} \\ \\ -\triangledown lng(\eta )